src/Pipit.System.Exp.fst
@@ -14,7 +14,7 @@ open Pipit.System.Det
 (* A system we get from translating an expression *)
 let xsystem (#t: table) (c: context t) (state: Type) (value: Type) = system (row c) state value
 (* Same, but deterministic *)
-// let xdsystem (#t: table) (c: context t) (state: Type) (value: Type) = dsystem (row c) state value
+let xdsystem (#t: table) (c: context t) (state: Type) (value: Type) = dsystem (row c) state value
 
 let xsystem_stepn
   (#tbl: table)
@@ -32,27 +32,122 @@ let rec state_of_exp (#t: table) (#c: context t) (#a: t.ty) (e: exp t c a): Tot 
   | XFby v e1 -> state_of_exp e1 & t.ty_sem a
   | XMu e1 -> state_of_exp e1
   | XLet b e1 e2 -> state_of_exp e1 & state_of_exp e2
-  | XCheck name e1 -> (t.ty_sem t.propty & state_of_exp e1)
+  | XCheck name e1 -> bool & state_of_exp e1
   // Contracts do not expose their body in abstract mode, so we only need state of rely and guar
   | XContract rely guar impl ->
-    state_of_exp rely & state_of_exp guar
+    (bool & bool) & (state_of_exp rely & state_of_exp guar)
 
 and state_of_exp_apps (#t: table) (#c: context t) (#a: funty t.ty) (e: exp_apps t c a): Tot Type (decreases e) =
   match e with
   | XPrim _ -> unit
-  | XApp f e -> state_of_exp_apps f & state_of_exp e
+  | XApp f e -> state_of_exp e & state_of_exp_apps f
+
+
+let rec dstate_of_exp (#t: table) (#c: context t) (#a: t.ty) (e: exp t c a): Tot Type (decreases e) =
+  match e with
+  | XBase _ -> unit
+  | XApps e1 -> dstate_of_exp_apps e1
+  | XFby v e1 -> dstate_of_exp e1 & t.ty_sem a
+  | XMu e1 -> dstate_of_exp e1
+  | XLet b e1 e2 -> dstate_of_exp e1 & dstate_of_exp e2
+  | XCheck name e1 -> bool & dstate_of_exp e1
+  | XContract rely guar impl ->
+    dstate_of_exp impl
+
+and dstate_of_exp_apps (#t: table) (#c: context t) (#a: funty t.ty) (e: exp_apps t c a): Tot Type (decreases e) =
+  match e with
+  | XPrim _ -> unit
+  | XApp f e -> dstate_of_exp e & dstate_of_exp_apps f
+
+
+let rec exp_is_deterministic (#t: table) (#c: context t) (#a: t.ty) (e: exp t c a): Tot bool (decreases e) =
+  match e with
+  | XBase _ -> true
+  | XApps e1 -> exp_apps_is_deterministic e1
+  | XFby v e1 -> exp_is_deterministic e1
+  | XMu e1 -> exp_is_deterministic e1
+  | XLet b e1 e2 -> exp_is_deterministic e1 && exp_is_deterministic e2
+  | XCheck name e1 -> exp_is_deterministic e1
+  // Contracts do not expose their body in abstract mode, so we only need state of rely and guar
+  | XContract rely guar impl ->
+    false
+
+and exp_apps_is_deterministic (#t: table) (#c: context t) (#a: funty t.ty) (e: exp_apps t c a): Tot bool (decreases e) =
+  match e with
+  | XPrim _ -> true
+  | XApp f e -> exp_apps_is_deterministic f && exp_is_deterministic e
+
+let lemma_state_dstate_det (#t: table) (#c: context t) (#a: t.ty) (e: exp t c a { exp_is_deterministic e }):
+  Lemma (state_of_exp e == dstate_of_exp e) =
+  admit ()
+
+
+let dsystem_of_exp_base
+  (#t: table) (#c: context t) (#a: t.ty)
+  (e: exp_base t c a { Causal.causal_base e }):
+    Tot (xdsystem c unit (t.ty_sem a)) (decreases e) =
+    match e with
+    | XVal v -> dsystem_const v
+    | XBVar x -> dsystem_map_input (fun i -> CR.index (context_sem c) i x)
+    | XVar x -> false_elim ()
+
+
+let rec dsystem_of_exp
+  (#t: table) (#c: context t) (#a: t.ty)
+  (e: exp t c a { Causal.causal e }):
+    Tot (xdsystem c (dstate_of_exp e) (t.ty_sem a)) (decreases e) =
+    match e with
+    | XBase e1 -> dsystem_of_exp_base e1
+    | XApps e1 ->
+      let t: dsystem (unit & row c) (dstate_of_exp_apps e1) (t.ty_sem a) = dsystem_of_exp_apps e1 (fun r i -> r) in
+      dsystem_with_input (fun s -> ((), s)) t
+    | XFby v e1 ->
+      dsystem_pre v (dsystem_of_exp e1)
+    | XMu e1 ->
+      let t' = dsystem_of_exp e1 in
+      dsystem_mu_causal #(row c) #(t.ty_sem a & row c) (t.val_default a) (fun i v -> (v, i)) t'
+    | XLet b e1 e2 ->
+      dsystem_let (fun i v -> (v, i)) (dsystem_of_exp e1) (dsystem_of_exp e2)
+    | XCheck name e1 ->
+      dsystem_check name (dsystem_of_exp e1)
+    | XContract rely guar impl ->
+      dsystem_of_exp impl
+
+and dsystem_of_exp_apps
+  (#t: table) (#c: context t) (#a: funty t.ty) (#res #inp: Type0)
+  (e: exp_apps t c a { Causal.causal_apps e })
+  (f: funty_sem t.ty_sem a -> inp -> res):
+    Tot (dsystem (inp & row c) (dstate_of_exp_apps e) res) (decreases e) =
+    match e with
+    | XPrim p -> dsystem_map_input  (fun i -> f (t.prim_sem p) (fst i))
+    | XApp e1 e2 ->
+      let arg = XApp?.arg e in
+      let ret = XApp?.ret e in
+      lemma_funty_sem_FTFun t.ty_sem arg ret;
+      let t1: dsystem ((t.ty_sem arg & inp) & row c) _ res = dsystem_of_exp_apps e1 (fun r i -> f (r (fst i)) (snd i)) in
+      let t2: xdsystem c _ (t.ty_sem arg) = dsystem_of_exp e2 in
+      let t2': dsystem (inp & row c) _ (t.ty_sem arg) = dsystem_with_input snd t2 in
+      dsystem_let (fun i v -> ((v, fst i), snd i)) t2' t1
+
+
 
 let rec system_of_exp
   (#t: table) (#c: context t) (#a: t.ty)
   (e: exp t c a { Causal.causal e }):
     Tot (xsystem c (state_of_exp e) (t.ty_sem a)) (decreases e) =
-  // if exp_is_function e then system_of_dsystem (dsystem_of_exp e)
-  // else
+  // PERF:TRANS: wrong complexity!
+  // This has the wrong complexity. We descend into the expression to check if it's deterministic, but each sub-call will also descend.
+  // The right way to do this is probably to create a datatype that can represent both xsystem and xdsystem, and have combinators to join them together.
+  if exp_is_deterministic e
+  then (
+    lemma_state_dstate_det e;
+    system_of_dsystem (dsystem_of_exp e))
+  else
     match e with
-    | XBase (XVal v) -> system_const v
-    | XBase (XBVar x) -> system_map (fun i -> CR.index (context_sem c) i x) system_input
-    | XBase (XVar x) -> false_elim ()
-    | XApps e1 -> system_of_exp_apps e1
+    | XBase e1 -> false_elim ()
+    | XApps e1 ->
+      let t: system (unit & row c) (state_of_exp_apps e1) (t.ty_sem a) = system_of_exp_apps e1 (fun r i -> r) in
+      system_with_input (fun s -> ((), s)) t
     | XFby v e1 ->
       system_pre v (system_of_exp e1)
     | XMu e1 ->
@@ -60,61 +155,26 @@ let rec system_of_exp
       system_mu #(row c) #(t.ty_sem a & row c) (fun i v -> (v, i)) t'
     | XLet b e1 e2 ->
       system_let (fun i v -> (v, i)) (system_of_exp e1) (system_of_exp e2)
-    // | XContract assm guar body arg ->
-    //   system_contract_instance (fun i b -> (b, ())) (fun i a b -> (a, (b, ())))
-    //     (system_bool_holds (system_of_exp assm))
-    //     (system_bool_holds (system_of_exp guar))
-    //     (system_of_exp arg)
     | XCheck name e1 ->
-      system_check t.propty_sem (t.propty_of_bool true) name (system_of_exp e1)
+      system_check name (system_of_exp e1)
     | XContract rely guar impl ->
-      admit ()
+      let tr = system_of_exp rely in
+      let tg = system_of_exp guar in
+      system_contract_instance tr tg
 
 and system_of_exp_apps
-  (#t: table) (#c: context t) (#a: funty t.ty)
-  (e: exp_apps t c a { Causal.causal_apps e }):
-    Tot (xsystem c (state_of_exp_apps e) (funty_sem t.ty_sem a)) (decreases e) =
-  // if exp_is_function e then system_of_dsystem (dsystem_of_exp e)
-  // else
+  (#t: table) (#c: context t) (#a: funty t.ty) (#res #inp: Type0)
+  (e: exp_apps t c a { Causal.causal_apps e })
+  (f: funty_sem t.ty_sem a -> inp -> res):
+    Tot (system (inp & row c) (state_of_exp_apps e) res) (decreases e) =
     match e with
-    | XPrim p -> system_const (t.prim_sem p)
+    | XPrim p -> system_map_input  (fun i -> f (t.prim_sem p) (fst i))
     | XApp e1 e2 ->
       let arg = XApp?.arg e in
       let ret = XApp?.ret e in
-      lemma_funty_sem_FTFun t.ty_sem (XApp?.arg e) (XApp?.ret e);
-      // assert_norm (Causal.causal_ (XApp e1 e2) ==> (Causal.causal e1 && Causal.causal e2));
-      let t1: xsystem c _ (funty_sem t.ty_sem (FTFun arg ret)) = system_of_exp_apps e1 in
+      lemma_funty_sem_FTFun t.ty_sem arg ret;
+      let t1: system ((t.ty_sem arg & inp) & row c) _ res = system_of_exp_apps e1 (fun r i -> f (r (fst i)) (snd i)) in
       let t2: xsystem c _ (t.ty_sem arg) = system_of_exp e2 in
-      system_ap2 t1 t2
-      // let t': xsystem c (state_of_exp_apps (XApp e1 e2)) (funty_sem t.ty_sem a) = system_ap2 t1 t2 in
+      let t2': system (inp & row c) _ (t.ty_sem arg) = system_with_input snd t2 in
+      system_let (fun i v -> ((v, fst i), snd i)) t2' t1
 
-
-(*
-let rec dsystem_of_exp (#t: table) (#c: context t) (e: exp t c 'a { Causal.causal e }):
-    Tot (xdsystem c (state_of_exp e) 'a) (decreases e) =
-  match e with
-  | XVal v -> dsystem_const v
-  | XPrim p -> dsystem_const (t.prim_sem p)
-  | XBVar x -> dsystem_map (fun i -> CR.index (context_sem c) i x) dsystem_input
-  | XVar x -> false_elim ()
-  | XApp e1 e2 ->
-    assert_norm (Causal.causal (XApp e1 e2) ==> (Causal.causal e1 && Causal.causal e2));
-    let t1 = dsystem_of_exp e1 in
-    let t2 = dsystem_of_exp e2 in
-    let t': xdsystem c (state_of_exp (XApp e1 e2)) 'a = dsystem_ap2 t1 t2 in
-    t'
-  | XFby v e1 ->
-    dsystem_pre v (dsystem_of_exp e1)
-  | XThen e1 e2 ->
-    dsystem_then (dsystem_of_exp e1) (dsystem_of_exp e2)
-  | XMu e1 ->
-    let t' = dsystem_of_exp e1 in
-    dsystem_mu_causal #(row c) #('a & row c) (t.val_default (XMu?.valty e)) (fun i v -> (v, i)) t'
-  | XLet b e1 e2 ->
-    dsystem_let (fun i v -> (v, i)) (dsystem_of_exp e1) (dsystem_of_exp e2)
-  | XCheck name e1 e2 ->
-    let t1 = dsystem_check t.propty_sem (t.propty_of_bool true) name (dsystem_of_exp e1) in
-    let t2 = dsystem_of_exp e2 in
-    let t': xdsystem c (state_of_exp (XCheck name e1 e2)) 'a = dsystem_let (fun i v -> i) t1 t2 in
-    t'
-*)
