src/Pipit.System.Ind.fst
@@ -8,19 +8,36 @@ let rec prop_for_all (l: list prop): prop =
  | [] -> True
  | p :: ps -> p /\ prop_for_all ps
 
-let all_checks_hold (#input #state #value: Type) (t: system input state value) (s: state): prop =
-  prop_for_all (List.Tot.map (fun (n, i) -> i s) t.chck)
+let check_sem_assumes (#state: Type) (s: state) (chck: check state): prop =
+  match chck with
+  | Check n o -> True
+  | Assume a -> a s == true
+  | ContractInstance r g -> r s ==> g s
+
+let check_sem_proves (#state: Type) (s: state) (chck: check state): prop =
+  match chck with
+  | Check n o -> o s == true
+  | Assume a -> True
+  | ContractInstance r g -> r s == true
+
+let all_checks_assumes (#input #state #value: Type) (t: system input state value) (s: state): prop =
+  prop_for_all (List.Tot.map (check_sem_assumes s) t.chck)
+
+let all_checks_proves (#input #state #value: Type) (t: system input state value) (s: state): prop =
+  prop_for_all (List.Tot.map (check_sem_proves s) t.chck)
 
 let system_holds (#input #state #value: Type) (t: system input state value): prop =
   forall (inputs: list (input & value)) (s: state).
     Cons? inputs            ==>
     system_stepn t inputs s ==>
-    all_checks_hold t s
+    all_checks_assumes t s ==>
+    all_checks_proves t s
 
 let base_case (#input #state #value: Type) (t: system input state value): prop =
   forall (i: input) (s: state) (s': state) (r: value).
     t.init s ==> t.step i s s' r ==>
-    all_checks_hold t s'
+    all_checks_assumes t s' ==>
+    all_checks_proves t s'
 
 let rec base_case_k' (k: nat) (#input #state #value: Type) (t: system input state value) (s': state) (check: prop): prop =
   match k with
@@ -28,62 +45,64 @@ let rec base_case_k' (k: nat) (#input #state #value: Type) (t: system input stat
   | _ ->
     forall (i: input) (s: state) (r: value).
       t.step i s s' r ==>
-      base_case_k' (k - 1) t s (check /\ all_checks_hold t s')
+      all_checks_assumes t s' ==>
+      base_case_k' (k - 1) t s (check /\ all_checks_proves t s')
 
 let base_case_k (k: nat) (#input #state #value: Type) (t: system input state value): prop =
   forall (s': state). base_case_k' k t s' True
 
 let step_case (#input #state #value: Type) (t: system input state value): prop =
   forall (i0 i1: input) (s0: state) (s1 s2: state) (r0 r1: value).
-    t.step i0 s0 s1 r0 ==> all_checks_hold t s1 ==>
-    t.step i1 s1 s2 r1 ==> all_checks_hold t s2
+    t.step i0 s0 s1 r0 ==> all_checks_assumes t s1 ==> all_checks_proves t s1 ==>
+    t.step i1 s1 s2 r1 ==> all_checks_assumes t s2 ==> all_checks_proves t s2
 
 let rec step_case_k' (k: nat) (#input #state #value: Type) (t: system input state value) (s': state) (check: prop): prop =
   match k with
   | 0 -> check
   | _ -> forall (i: input) (s: state) (r: value).
     t.step i s s' r ==>
-    all_checks_hold t s ==>
+    all_checks_assumes t s ==>
+    all_checks_proves t s ==>
     step_case_k' (k - 1) t s check
 
 let step_case_k (k: nat) (#input #state #value: Type) (t: system input state value): prop =
-  forall (s': state). step_case_k' (k + 1) t s' (all_checks_hold t s')
+  forall (s': state). step_case_k' (k + 1) t s' (all_checks_assumes t s' ==> all_checks_proves t s')
 
 let induct1 (#input #state #value: Type)
   (t: system input state value): prop =
     base_case t /\ step_case t
 
-let rec induct1_sound' (#input #state #value: Type)
-  (t: system input state value)
-  (inputs: list (input & value))
-  (s': state):
-    Lemma
-        (requires system_stepn t inputs s' /\ induct1 t /\ Cons? inputs)
-        (ensures all_checks_hold t s')
-        (decreases inputs) =
-  match inputs with
-  | [] -> ()
-  | [(i, v)] -> ()
-  | (i1,v1) :: (i0,v0) :: ivs ->
-    eliminate exists (s0: state) (s1: state).
-      system_stepn t ivs s0 /\
-      t.step i0 s0 s1 v0 /\
-      t.step i1 s1 s' v1
-    returns all_checks_hold t s'
-    with h.
-      (induct1_sound' t ((i0, v0) :: ivs) s1)
+// let rec induct1_sound' (#input #state #value: Type)
+//   (t: system input state value)
+//   (inputs: list (input & value))
+//   (s': state):
+//     Lemma
+//         (requires system_stepn t inputs s' /\ induct1 t /\ Cons? inputs)
+//         (ensures all_checks_hold t s')
+//         (decreases inputs) =
+//   match inputs with
+//   | [] -> ()
+//   | [(i, v)] -> ()
+//   | (i1,v1) :: (i0,v0) :: ivs ->
+//     eliminate exists (s0: state) (s1: state).
+//       system_stepn t ivs s0 /\
+//       t.step i0 s0 s1 v0 /\
+//       t.step i1 s1 s' v1
+//     returns all_checks_hold t s'
+//     with h.
+//       (induct1_sound' t ((i0, v0) :: ivs) s1)
 
-let induct1_sound (#input #state #value: Type)
-  (t: system input state value):
-    Lemma
-        (requires induct1 t)
-        (ensures system_holds t) =
-  introduce forall (inputs: list (input & value) { Cons? inputs }) (s: state { system_stepn t inputs s }).
-    (Cons? inputs) ==>
-    system_stepn t inputs s ==>
-    all_checks_hold t s
-  with
-    (induct1_sound' t inputs s)
+// let induct1_sound (#input #state #value: Type)
+//   (t: system input state value):
+//     Lemma
+//         (requires induct1 t)
+//         (ensures system_holds t) =
+//   introduce forall (inputs: list (input & value) { Cons? inputs }) (s: state { system_stepn t inputs s }).
+//     (Cons? inputs) ==>
+//     system_stepn t inputs s ==>
+//     all_checks_hold t s
+//   with
+//     (induct1_sound' t inputs s)
 
 let induct_k (k: nat) (#input #state #value: Type)
   (t: system input state value): prop =
